DG Discretization of the Variable Coefficient Poisson Equation

Buğrahan Temür

February 2023

Start with the model problem with a tensor-valued continuous variable coefficient $\lambda=\lambda\left(x\right)$

$$-\nabla \cdot (\boldsymbol{\lambda} \nabla u) = f \quad \text{in } \Omega , \qquad (1)$$

$$u = g \qquad \text{on } \Gamma^D, \tag{2}$$

$$\nabla u \cdot \boldsymbol{n} = h \quad \text{on } \Gamma^N.$$
(3)

Introduce an auxiliary variable σ to acquire two first-order equations

$$-\nabla \cdot (\boldsymbol{\lambda}\boldsymbol{\sigma}) = f , \qquad (4)$$

$$\boldsymbol{\sigma} = \nabla u \ . \tag{5}$$

Multiply Eq. 5 with the variable coefficient λ , then multiply both equations with appropriate test functions and integrate over cells

$$(v_h, -\nabla \cdot (\boldsymbol{\lambda}\boldsymbol{\sigma}_h))_{\Omega_e} = (v_h, f)_{\Omega_e} \quad , \tag{6}$$

$$(\boldsymbol{\tau}_h, \boldsymbol{\lambda}\boldsymbol{\sigma}_h)_{\Omega_e} = (\boldsymbol{\tau}_h, \boldsymbol{\lambda}\nabla u_h)_{\Omega_e}$$
 (7)

Integrate the LHS of Eq. 6 by parts and introduce the numerical flux $\pmb{\sigma}_h^*$ of the auxiliary variable

$$(\nabla v_h, \boldsymbol{\lambda}\boldsymbol{\sigma}_h)_{\Omega_e} - (v_h, \boldsymbol{\sigma}_h^* \boldsymbol{\lambda}^T \boldsymbol{n})_{\partial \Omega_e} = (v_h, f)_{\Omega_e} \quad . \tag{8}$$

Integrate the RHS of Eq. 7 by parts and introduce the numerical flux u_h^\ast of the solution

$$(\boldsymbol{\tau}_h, \boldsymbol{\lambda}\boldsymbol{\sigma}_h)_{\Omega_e} = -\left(\nabla \cdot (\boldsymbol{\tau}_h \boldsymbol{\lambda}), u_h\right)_{\Omega_e} + (\boldsymbol{\tau}_h, \boldsymbol{\lambda} u_h^* \boldsymbol{n})_{\partial \Omega_e} \quad . \tag{9}$$

As the next step to get to the primal formulation, integrate this once more by parts to obtain

$$(\boldsymbol{\tau}_h, \boldsymbol{\lambda}\boldsymbol{\sigma}_h)_{\Omega_e} = (\boldsymbol{\tau}_h, \boldsymbol{\lambda}\nabla u_h)_{\Omega_e} - (\boldsymbol{\tau}_h, \boldsymbol{\lambda}(u_h - u_h^*)\boldsymbol{n})_{\partial\Omega_e} \quad . \tag{10}$$

Set $\boldsymbol{\tau}_h = \nabla v_h$ and substitute Eq. 10 for the first term in Eq. 8, which gives the primal form

$$(\nabla v_h, \boldsymbol{\lambda} \nabla u_h)_{\Omega_e} - (\nabla v_h, \boldsymbol{\lambda} (u_h - u_h^*) \boldsymbol{n})_{\partial \Omega_e} - (v_h, \boldsymbol{\sigma}_h^* \boldsymbol{\lambda}^T \boldsymbol{n})_{\partial \Omega_e} - (v_h, f)_{\Omega_e} = 0 .$$

$$(11)$$

Define the fluxes according to the SIPG method with the average and jump operators

$$u_h^* = \{\!\{u_h\}\!\} , \qquad (12)$$

$$\boldsymbol{\sigma}_h^* = \{\!\{\nabla u_h\}\!\} - \tau \llbracket u_h \rrbracket \quad . \tag{13}$$

Substitute the fluxes to finally get

$$(\nabla v_h, \boldsymbol{\lambda} \nabla u_h)_{\Omega_e} - \frac{1}{2} (\nabla v_h, \boldsymbol{\lambda} \llbracket u_h \rrbracket)_{\partial \Omega_e} - (v_h, \{\{\nabla u_h\}\} \boldsymbol{\lambda}^T \boldsymbol{n})_{\partial \Omega_e} - (v_h, \tau \llbracket u_h \rrbracket \boldsymbol{\lambda}^T \boldsymbol{n})_{\partial \Omega_e} - (v_h, f)_{\Omega_e} = 0.$$
(14)